Spec/RefinementObligation.s.dfy
@@ -1,0 +1,63 @@
+abstract module UIOpIfc {
+  // transition labels enforce correspondence between low-level trusted ABI & upper-level semantics
+  type UIOp(!new,==)
+}
+
+abstract module StateMachineIfc(uiopifc: UIOpIfc) {
+  type Constants(!new,==)
+  type Variables(!new,==)
+
+  predicate Init(c: Constants, v: Variables)
+
+  predicate Next(c: Constants, v: Variables, v': Variables, uiop: uiopifc.UIOp)
+}
+
+abstract module RefinesIfc(
+  uiopifc: UIOpIfc, lower: StateMachineIfc(uiopifc), upper: StateMachineIfc(uiopifc)) {
+  function Iconstants(lc: lower.Constants) : (uc: upper.Constants)
+
+  function I(lc: lower.Constants, lv: lower.Variables) : (uv: upper.Variables)
+
+  // Give the prover an opprotunity to constrain the state space over which refinement works.
+  // In TLA terms, we're enabling this proof strategy: Init && []Next ==> []Inv ==> []Refines
+  predicate Inv(lc: lower.Constants, lv: lower.Variables)
+
+  // That Inv-constrained state space has to be big enough to include all valid lower-behaviors
+  lemma InvInductive(lc: lower.Constants, lv: lower.Variables, lv': lower.Variables, uiop: uiopifc.UIOp)
+    ensures lower.Init(lc, lv) ==> Inv(lc, lv)
+    ensures Inv(lc, lv) && lower.Next(lc, lv, lv', uiop) ==> Inv(lc, lv')
+
+  // Every time the lower machine takes a next step labeled with uiop, the upper state machine
+  // takes a correspondingly-labeled step.
+  lemma Refines(lc: lower.Constants, lv: lower.Variables, lv': lower.Variables, uiop: uiopifc.UIOp)
+    ensures Inv(lc, lv) && lower.Next(lc, lv, lv', uiop)
+      ==> upper.Next(Iconstants(lc), I(lc, lv), I(lc, lv'), uiop)
+}
+
+// For now, while we're only going down into atomic state machines, we want to prove
+// statements of this form:
+//module ImplementationObligation(implementation: StateMachineIfc) refines RefinesIfc(CrashTolerantUIOp(MapSpec), implementation, CrashTolerantMapSpecMod ) {}
+
+// Eventually, we'll have some .s runtime framework for a single-threaded event loop.
+// That framework will require refinement from the heap states to the top-level state
+// machine, and it'll be placed correctly to enforce uiop correpsondence.
+//module MainIfc(implStateMachine: ) {
+//  function Iconstants() 
+//
+//  function Iheap() 
+//    reads *
+//
+//  method setup()
+//    ensures 
+//
+//  method handle()
+//}
+
+//module ImplementationObligation(implementation: MainIfc) refines RefinesIfc(implementation, CrashTolerantMapSpecMod) { }
+
+// Build system will enforce this single line, the one line that is both trusted
+// and includes the implementation by reference.
+// Notice that this line can be used by every instance of this methodology:
+// RefinementObligation is defined by "player one" (in a trusted .s file);
+// Main is defined by "player two" (in a verified file tree).
+//module ConcreteRefinementObligation refines ImplementationObligation(Main)
