Splinter/Paged/Bundle.i.dfy
@@ -1,11 +1,14 @@
 include "AbstractJournal.i.dfy"
 include "AbstractMap.i.dfy"
 include "PagedJournal.i.dfy"
+include "../../Spec/RefinementObligation.s.dfy"
 
 // Hey look, this abstract journal satisfies the refinement.
-module AbstractJournalRefinement refines CoordinationSystemRefinement(AbstractJournal, AbstractMap) {
-}
+module AbstractJournalRefinement refines CoordinationSystemRefinement(AbstractJournal, AbstractMap) { }
+
+module ImplementationObligation(implementation: StateMachineIfc) refines RefinesIfc(implementation, CrashTolerantMapSpecMod) { }
+
+module ConcreteRefinementProof refines ImplementationObligation(AbstractJournalRefinement) { }
 
 // Ooh, and so does this Paged journal
-module PagedJournalRefinement refines CoordinationSystemRefinement(PagedJournal, AbstractMap) {
-}
+module PagedJournalRefinement refines CoordinationSystemRefinement(PagedJournal, AbstractMap) { }
